Delete duplicate code in Total.lean

LeanSorting/Total.lean
@@ -1,15 +1,13 @@
 import Mathlib.Data.Nat.ModEq
 import Batteries.Classes.Order
 import Init.Data.Array.Lemmas
+import LeanSorting.Slice.Basic
 
 open Batteries
 
 theorem Nat.lt_of_lt_le {a b c : ℕ} (h : a < b) : b ≤ c → a < c := by omega
 theorem Nat.lt_of_le_lt {a b c : ℕ} (h : a ≤ b) : b < c → a < c := by omega
 theorem Nat.sub_succ_lt_sub_of_lt {a b : ℕ} (h : a < b) : b - a.succ < b - a := by omega
-
-def Nat.in_range (n : ℕ) (low high : ℕ) : Prop := n ≥ low ∧ n < high
-def Nat.adjacent_in_range (n m low high : ℕ) : Prop := n.succ = m ∧ n ≥ low ∧ m < high
 
 variable
   {α : Type}
@@ -22,119 +20,6 @@ variable
   {low high low₁ high₁ low₂ high₂ ptr ptr₁ ptr₂ mid : ℕ}
   (s : @Slice α arr low high)
   (s_i : @Slice α arr_i low_i high_i)
-
-structure Slice (arr : Array α) (low high : ℕ) : Prop where
-  low_le_high : low ≤ high
-  high_le_size : high ≤ arr.size
-
--- def Slice.mkEmpty (arr : Array α) (low high : ℕ) (h_empty : low = high) : Slice arr low high :=
---   { low_le_high := h_empty,
---     high_le_size :=
-
---   }
-
--- inductive Slice.pairwise : Slice arr low high → Prop where
---   | empty : ∀ {s : Slice arr low high}, low = high → s.pairwise
---   |
-
-structure SlicePtrExclusive (arr : Array α) (low high : ℕ) (ptr : ℕ)
-    extends Slice arr low high : Prop where
-  ptr_ge_low : ptr ≥ low
-  ptr_lt_high : ptr < high
-
-def SlicePtrExclusive.ptr_lt_size (s : SlicePtrExclusive arr low high ptr) : ptr < arr.size :=
-  Nat.lt_of_lt_le s.ptr_lt_high s.high_le_size
-
-structure SlicePtrInclusive (arr : Array α) (low high : ℕ) (ptr : ℕ)
-    extends Slice arr low high : Prop where
-  ptr_ge_low : ptr ≥ low
-  ptr_le_high : ptr ≤ high
-
-def SlicePtrInclusive.ptr_le_size (s : SlicePtrInclusive arr low high ptr) : ptr ≤ arr.size :=
-  Nat.le_trans s.ptr_le_high s.high_le_size
-
--- In a slice [a, b, c, d, e, >f<, g] with pointer at 'f', the left half is [a, b, c, d, e].
-def SlicePtrInclusive.left (s : SlicePtrInclusive arr low high ptr) : Slice arr low ptr :=
-  { low_le_high := s.ptr_ge_low
-    high_le_size := Nat.le_trans s.ptr_le_high s.high_le_size
-  }
-
-def SlicePtrInclusive.right (s : SlicePtrInclusive arr low high ptr) : Slice arr ptr high :=
-  { low_le_high := s.ptr_le_high
-    high_le_size := s.high_le_size
-  }
-
-def Slice.swap_arr
-    (s : Slice arr low high)
-    (size_eq : arr.size = aux.size)
-    : Slice aux low high :=
-  { s with high_le_size := by rw [← size_eq]; exact s.high_le_size }
-
-def SlicePtrExclusive.swap_arr
-    (s : SlicePtrExclusive arr low high ptr)
-    (size_eq : arr.size = aux.size)
-    : SlicePtrExclusive aux low high ptr :=
-  { s with
-    high_le_size := by rw [← size_eq]; exact s.high_le_size
-  }
-
-def SlicePtrInclusive.swap_arr
-    (s : SlicePtrInclusive arr low high ptr)
-    (size_eq : arr.size = aux.size)
-    : SlicePtrInclusive aux low high ptr :=
-  { s with
-    high_le_size := by rw [← size_eq]; exact s.high_le_size
-  }
-
-def SlicePtrExclusive.next
-    (s : SlicePtrExclusive arr low high ptr)
-    : SlicePtrInclusive arr low high ptr.succ :=
-  { s with
-    ptr_ge_low := by have := s.ptr_ge_low; omega,
-    ptr_le_high := s.ptr_lt_high,
-  }
-
-def SlicePtrInclusive.mkExclusive
-    (s : SlicePtrInclusive arr low high ptr)
-    (ptr_lt_high : ptr < high)
-    : SlicePtrExclusive arr low high ptr :=
-  { s with ptr_lt_high }
-
-def Slice.sorted [Batteries.LawfulOrd α] (_s : Slice arr low high) : Prop :=
-  ∀ (i₁ i₂ : Fin arr.size)
-    (_adjacent_in_range : i₁.val.adjacent_in_range i₂ low high),
-      Ord.compare arr[i₁] arr[i₂] ≠ Ordering.gt
-
--- def Slice.sorted₂ {arr : Array α} {low high : ℕ} (s : Slice arr low high) : Prop :=
---   (low_succ_lt_high : low.succ < high) →
---     let high_le_size := s.high_le_size
---     let s' : Slice arr low.succ high := {
---       low_le_high := by omega
---       high_le_size := by omega
---     }
---     let x := arr[low]
---     let y := arr[low.succ]
---     let le := Ord.compare x y ≠ Ordering.gt
---     le ∧ Slice.sorted₂ s'
-
--- theorem Slice.sorted_of_sorted₂ : s.sorted₂ → s.sorted := by
---   sorry
-
--- theorem Slice.sorted₂_of_sorted : s.sorted → s.sorted₂ := by
---   sorry
-
--- theorem Slice.sorted_iff_sorted₂ : s.sorted ↔ s.sorted₂ := by
---   apply Iff.intro
---   . exact s.sorted₂_of_sorted
---   . exact s.sorted_of_sorted₂
-
--- A slice, s₁, is less than or equal to a slice s₂ if no element of s₁ is greater
--- than an element of s₂.
-def Slice.le (_s₁ : Slice arr₁ low₁ high₁) (_s₂ : Slice arr₂ low₂ high₂) : Prop :=
-  ∀ (i₁ : Fin arr₁.size) (i₂ : Fin arr₂.size),
-      i₁.val.in_range low₁ high₁
-    ∧ i₂.val.in_range low₂ high₂
-    → Ord.compare arr₁[i₁] arr₂[i₂] ≠ Ordering.gt
 
 structure H₁ (arr aux : Array α) (low mid high ptr₁ ptr₂ : ℕ) : Prop where
   slice₁ : SlicePtrInclusive arr low mid ptr₁
@@ -165,10 +50,10 @@ def H₂.mkH₃
     have i_lt_high : i < high := by
       have := h₂.i_def
       omega
-    exact h₂.slice_i.mkExclusive i_lt_high
+    exact h₂.slice_i.make_exclusive i_lt_high
   { h₂ with
-    slice₁_exclusive := h₂.slice₁.mkExclusive ptr₁_ptr₂_in_bounds.left,
-    slice₂_exclusive := h₂.slice₂.mkExclusive ptr₁_ptr₂_in_bounds.right,
+    slice₁_exclusive := h₂.slice₁.make_exclusive ptr₁_ptr₂_in_bounds.left,
+    slice₂_exclusive := h₂.slice₂.make_exclusive ptr₁_ptr₂_in_bounds.right,
     slice_i_exclusive
   }
 
@@ -183,214 +68,6 @@ def H₃.ptr₁_lt_arr_size (h₃ : H₃ arr aux low mid high ptr₁ ptr₂ i) :
 def H₃.ptr₂_lt_arr_size (h₃ : H₃ arr aux low mid high ptr₁ ptr₂ i) : ptr₂ < arr.size :=
   have s := h₃.slice₂_exclusive
   Nat.le_trans s.ptr_lt_high s.high_le_size
-
--- -- If an array is modified, but the element changed is outside the slice on the
--- -- right, then none of the elements in the slice changed, thus it is still sorted.
--- def Slice.sorted_outside_write_sorted
---     {arr : Array α}
---     {low high : ℕ}
---     (s : Slice arr low high)
---     (s_sorted : s.sorted)
---     {arr' : Array α}
---     {i : Fin arr.size}
---     {a : α}
---     {i_ge_high : i ≥ high}
---     {arr'_def : arr' = arr.set i a}
---     : have s' : Slice arr' low high :=
---         { low_le_high := s.low_le_high,
---           high_le_size := by simp [arr'_def]; exact s.high_le_size
---         }
---       s'.sorted := by
---   intro s'
---   unfold Slice.sorted
---   intro i₁' i₂' adjacent_in_bounds'
---   unfold Slice.sorted at s_sorted
---   have i₁'_lt_arr_size : i₁' < arr.size := by omega
---   have i₂'_lt_arr_size : i₂' < arr.size := by omega
---   let i₁ : Fin arr.size := ⟨i₁', i₁'_lt_arr_size⟩
---   let i₂ : Fin arr.size := ⟨i₂', i₂'_lt_arr_size⟩
---   have i₁'_eq_i₁ : i₁'.val = i₁.val := by rfl
---   have i₂'_eq_i₂ : i₂'.val = i₂.val := by rfl
---   rw [i₁'_eq_i₁, i₂'_eq_i₂] at adjacent_in_bounds'
---   have h := s_sorted i₁ i₂ adjacent_in_bounds'
---   simp [arr'_def]
---   have i_ne_i₁' : i.val ≠ i₁' := by omega
---   have i_ne_i₂' : i.val ≠ i₂' := by omega
---   have set_get₁ := arr.get_set_ne i a i₁'_lt_arr_size i_ne_i₁'
---   have set_get₂ := arr.get_set_ne i a i₂'_lt_arr_size i_ne_i₂'
---   rw [set_get₁, set_get₂]
---   exact h
-
-def Slice.le_elem (s : Slice arr low high) (a : α) : Prop :=
-  ∀ (i : ℕ) (in_bounds : i ≥ low ∧ i < high),
-    have high_le_size := s.high_le_size
-    Ord.compare arr[i] a ≠ Ordering.gt
-
-def Slice.ge_elem (s : Slice arr low high) (a : α) : Prop :=
-  ∀ (i : ℕ) (in_bounds : i ≥ low ∧ i < high),
-    have high_le_size := s.high_le_size
-    Ord.compare a arr[i] ≠ Ordering.gt
-
-def Slice.le_elem_of_le
-    (s₁ : Slice arr₁ low₁ high₁)
-    {s₂ : Slice arr₂ low₂ high₂}
-    (s₁_le_s₂ : s₁.le s₂)
-    (ptr_in_bounds₂ : ptr ≥ low₂ ∧ ptr < high₂)
-    : have high_le_size := s₂.high_le_size
-      s₁.le_elem arr₂[ptr] := by
-  intro high_le_size
-  unfold Slice.le_elem
-  intro i in_bounds high_le_size
-  unfold Slice.le at s₁_le_s₂
-  have i_lt_arr₁_size : i < arr₁.size := by omega
-  have ptr_lt_arr₂_size : ptr < arr₂.size := by omega
-  have h : i.in_range low₁ high₁ ∧ ptr.in_range low₂ high₂ := by
-    simp [Nat.in_range]
-    omega
-  exact s₁_le_s₂ ⟨i, i_lt_arr₁_size⟩ ⟨ptr, ptr_lt_arr₂_size⟩ h
-
-theorem not_gt_of_compare_same {a : α} : compare a a ≠ Ordering.gt := by
-  have compare_refl : compare a a = .eq := by exact OrientedCmp.cmp_refl
-  intro compare_eq_gt
-  have : Ordering.eq = Ordering.gt := by rw [← compare_refl, ← compare_eq_gt]
-  contradiction
-
-def Slice.ge_elem_low_of_sorted
-    (s_sorted : s.sorted)
-    (nonempty : low < high)
-    : by have := s.high_le_size
-         exact s.ge_elem arr[low]
-    := by
-  simp [Slice.ge_elem]
-  intro i in_bounds
-  simp [Slice.sorted] at s_sorted
-  have := s.low_le_high
-  have := s.high_le_size
-  let rec loop (i : ℕ) (in_bounds : i ≥ low ∧ i < high)
-      : compare arr[low] arr[i] ≠ Ordering.gt := by
-    if i_eq_low : i = low then
-      simp [i_eq_low]
-      exact not_gt_of_compare_same
-    else
-      let j := i - 1
-      have j_in_bounds : j ≥ low ∧ j < high := by omega
-      have ih := loop j j_in_bounds
-      let j_f : Fin arr.size := ⟨j, by omega⟩
-      let i_f : Fin arr.size := ⟨i, by omega⟩
-      have adj : j_f.val.adjacent_in_range i_f low high := by
-        simp [Nat.adjacent_in_range]
-        omega
-      have h := s_sorted j_f i_f adj
-      exact TransCmp.le_trans ih h
-  exact loop i in_bounds
-
-def Slice.ge_elem_low_succ_of_sorted
-    (s_sorted : s.sorted)
-    (nonempty : low < high)
-    (s' : Slice arr low.succ high)
-    : by have := s.high_le_size
-         exact s'.ge_elem arr[low]
-    := by
-  have h := s.ge_elem_low_of_sorted s_sorted nonempty
-  simp [Slice.ge_elem]
-  intro i in_bounds
-  simp [Slice.ge_elem] at h
-  have i_in_bounds : low ≤ i ∧ i < high := by omega
-  exact h i i_in_bounds
-
-set_option pp.proofs true
-
-def Slice.sorted_after_sorted_push
-    (s : Slice arr low high)
-    (s_sorted : s.sorted)
-    (high_lt_size : high < arr.size)
-    (arr'_def : arr' = arr.set ⟨high, high_lt_size⟩ a)
-    (s' : Slice arr' low high.succ)
-    (s_le_elem_a : s.le_elem a)
-    : s'.sorted := by
-  unfold Slice.sorted
-  intro i₁' i₂' adjacent_in_range'
-  simp [Nat.adjacent_in_range] at adjacent_in_range'
-  by_cases i₂'_eq_high : i₂' = high
-  . simp [i₂'_eq_high, arr'_def]
-    have i₁'_lt_arr_size : i₁'.val < arr.size := by omega
-    have high_ne_i₁' : high ≠ i₁' := by omega
-    have i₁'_same := arr.get_set_ne ⟨high, high_lt_size⟩ a i₁'_lt_arr_size high_ne_i₁'
-    rw [i₁'_same]
-    have in_bounds : i₁'.val.in_range low high := by simp [Nat.in_range]; omega
-    unfold Slice.le_elem at s_le_elem_a
-    exact s_le_elem_a i₁' in_bounds
-  . unfold Slice.sorted at s_sorted
-    have i₁'_lt_arr_size : i₁'.val < arr.size := by omega
-    have i₂'_lt_arr_size : i₂'.val < arr.size := by omega
-    simp [arr'_def]
-    have high_ne_i₁' : high ≠ i₁' := by omega
-    have high_ne_i₂' : high ≠ i₂' := by omega
-    have i₁'_same := arr.get_set_ne ⟨high, high_lt_size⟩ a i₁'_lt_arr_size high_ne_i₁'
-    have i₂'_same := arr.get_set_ne ⟨high, high_lt_size⟩ a i₂'_lt_arr_size high_ne_i₂'
-    simp [i₁'_same, i₂'_same]
-    let i₁ : Fin arr.size := ⟨i₁', i₁'_lt_arr_size⟩
-    let i₂ : Fin arr.size := ⟨i₂', i₂'_lt_arr_size⟩
-    have i₁_def : i₁ = ⟨i₁', i₁'_lt_arr_size⟩ := by rfl
-    have i₁_eq_i₁' : i₁' = i₁.val := by rw [i₁_def]
-    have adjacent_in_range : i₁.val.adjacent_in_range i₂ low high := by
-      simp [Nat.adjacent_in_range, i₂'_eq_high]
-      omega
-    exact s_sorted i₁ i₂ adjacent_in_range
-
-def SlicePtrInclusive.sorted_of_right_sorted
-    (s : SlicePtrInclusive arr low high ptr)
-    (s_sorted : s.sorted)
-    : s.right.sorted := by
-  unfold Slice.sorted at *
-  intro i₁ i₂ adjacent_in_range
-  have adjacent_in_range' : i₁.val.adjacent_in_range i₂ low high := by
-    unfold Nat.adjacent_in_range at *
-    have := s.ptr_ge_low
-    omega
-  exact s_sorted i₁ i₂ adjacent_in_range'
-
-def Slice.le_of_swap_ends_le
-    {aux : Slice arr₁ low₁ high₁}
-    {arr : Slice arr₂ low₂ high₂}
-    (arr_sorted : arr.sorted)
-    (aux_le_arr : aux.le arr)
-    (high₁_lt_arr₁_size : high₁ < arr₁.size)
-    (low₂_lt_arr₂_size : low₂ < arr₂.size)
-    (arr₁'_def : arr₁' = arr₁.set ⟨high₁, high₁_lt_arr₁_size⟩ arr₂[low₂])
-    (s₁' : Slice arr₁' low₁ high₁.succ)
-    (s₂' : Slice arr₂ low₂.succ high₂)
-    (size_eq : arr₂.size = arr₁.size)
-    : s₁'.le s₂' := by
-  unfold Slice.le
-  intro i₁' i₂' i₂'_i₂'_in_range
-  unfold Nat.in_range at i₂'_i₂'_in_range
-  unfold Slice.le at aux_le_arr
-  by_cases h : i₁' = high₁
-  . simp [h, arr₁'_def]
-    rw [Slice.sorted] at arr_sorted
-    have low₂_lt_high₂ : low₂ < high₂ := by omega
-    have x := arr.ge_elem_low_succ_of_sorted arr_sorted low₂_lt_high₂ s₂'
-    simp [Slice.ge_elem] at x
-    have i₂'_in_range : low₂ + 1 ≤ ↑i₂' ∧ ↑i₂' < high₂ := by omega
-    have x2 := x i₂' i₂'_in_range
-    exact x2
-  . have i₁'_lt_arr₁_size : i₁'.val < arr₁.size := by omega
-    have i₂'_lt_arr₂_size : i₂'.val < arr₂.size := by omega
-    let i₁ : Fin arr₁.size := ⟨i₁', i₁'_lt_arr₁_size⟩
-    let i₂ : Fin arr₂.size := ⟨i₂', i₂'_lt_arr₂_size⟩
-    simp [arr₁'_def]
-    have high_ne_i₁' : high₁ ≠ i₁' := by omega
-    have i₁'_same := arr₁.get_set_ne
-      ⟨high₁, high₁_lt_arr₁_size⟩
-      arr₂[low₂]
-      i₁'_lt_arr₁_size
-      high_ne_i₁'
-    simp [i₁'_same]
-    have i₁_i₂_in_range : i₁.val.in_range low₁ high₁ ∧ i₂.val.in_range low₂ high₂ := by
-      simp [Nat.in_range]
-      omega
-    exact aux_le_arr i₁ i₂ i₁_i₂_in_range
 
 def slice_ptr_le_of_succ
     (slice₁_ptr : SlicePtrExclusive arr low high ptr₁)
@@ -418,11 +95,11 @@ def H₃.nextLeft
     := by
   intro ptr₁_lt_arr_size aux'
   have aux'_def : aux' = aux.set ⟨i, h₃.i_lt_aux_size⟩ arr[ptr₁] := by rfl
-  have slice₁ := h₃.slice₁_exclusive.next
+  have slice₁ := h₃.slice₁_exclusive.increment_ptr
   have size_eq : arr.size = aux'.size := by simp [aux']; exact h₃.size_eq
   have aux_size_eq : aux.size = aux'.size := by simp [aux']
   have slice_i : SlicePtrInclusive aux' low high i.succ :=
-    h₃.slice_i_exclusive.next.swap_arr aux_size_eq
+    h₃.slice_i_exclusive.increment_ptr.swap_array aux_size_eq
   have i_def : i.succ = ptr₁.succ + ptr₂ - mid := by
     have := h₃.i_def
     have := h₃.slice₂.ptr_ge_low
